\newpage
\thispagestyle{empty}
{\flushleft Solutions to Homework Set 1}
{\bf \flushleft 1.}   $ \stackrel{\rightarrow}{A} \textup{x} \stackrel{\rightarrow}{B} = - (\stackrel{\rightarrow}{B} \textup{x} \stackrel{\rightarrow}{A})$.
{\flushleft \bf vector=vector}

 $[ \stackrel{\rightarrow}{A} \textup{x} \stackrel{\rightarrow}{B}]_i=
 \epsilon_{ijk}A_jB_k= - \epsilon_{ikj}B_kA_j = -[ \stackrel{\rightarrow}{B} \textup{x} \stackrel{\rightarrow}{A}]_i$
\vspace{.1in}

{\bf \flushleft 2.} $(\stackrel{\rightarrow}{A} \textup{x} \stackrel{\rightarrow}{B})\cdot (\stackrel{\rightarrow}{C} \textup{x} \stackrel{\rightarrow}{D})=(\stackrel{\rightarrow}{A} \cdot \stackrel{\rightarrow}{C})(\stackrel{\rightarrow}{B} \cdot \stackrel{\rightarrow}{D} ) -
(\stackrel{\rightarrow}{A} \cdot \stackrel{\rightarrow}{D})(\stackrel{\rightarrow}{B} \cdot \stackrel{\rightarrow}{C} )$
{\flushleft \bf scalar=scalar}
\begin{eqnarray*}
(\stackrel{\rightarrow}{A} \textup{x} \stackrel{\rightarrow}{B})
\cdot (\stackrel{\rightarrow}{C} \textup{x} \stackrel{\rightarrow}{D})&=&
\epsilon_{ijk}A_jB_k\epsilon_{ilm}C_lD_m\\
&=&\epsilon_{jki}\epsilon_{lmi}A_jB_kC_lD_m\\
&=&(\delta_{jl}\delta_{km}-\delta_{jm}\delta_{kl})A_jB_kC_lD_m\\
&=&A_jB_kC_jD_k-A_jB_kC_kD_j\\
&=&(\stackrel{\rightarrow}{A} \cdot \stackrel{\rightarrow}{C})(\stackrel{\rightarrow}{B} \cdot \stackrel{\rightarrow}{D} ) -
(\stackrel{\rightarrow}{A} \cdot \stackrel{\rightarrow}{D})(\stackrel{\rightarrow}{B} \cdot \stackrel{\rightarrow}{C} )
\end{eqnarray*}

\vspace{.1in}
{\bf \flushleft 3.} $(\stackrel{\rightarrow}{A} \textup{x} \stackrel{\rightarrow}{B})\textup{x} (\stackrel{\rightarrow}{C} \textup{x} \stackrel{\rightarrow}{D})= [\stackrel{\rightarrow}{A} , \stackrel{\rightarrow}{C} , \stackrel{\rightarrow}{D}] \stackrel{\rightarrow}{B} -
[\stackrel{\rightarrow}{B} , \stackrel{\rightarrow}{C} , \stackrel{\rightarrow}{D}] \stackrel{\rightarrow}{A}$
{\flushleft \bf vector=vector}
\begin{eqnarray*}
[(\stackrel{\rightarrow}{A} \textup{x} \stackrel{\rightarrow}{B})\textup{x} (\stackrel{\rightarrow}{C} \textup{x} \stackrel{\rightarrow}{D})]_i&=&
\epsilon_{ijk}(\stackrel{\rightarrow}{A} \textup{x} \stackrel{\rightarrow}{B})_j (\stackrel{\rightarrow}{C} \textup{x} \stackrel{\rightarrow}{D})_k\\
&=&\epsilon_{ijk}\epsilon_{jlm}A_lB_m (\stackrel{\rightarrow}{C} \textup{x} \stackrel{\rightarrow}{D})_k\\
&=&\epsilon_{kij}\epsilon_{lmj}A_lB_m (\stackrel{\rightarrow}{C} \textup{x} \stackrel{\rightarrow}{D})_k\\
&=&(\delta_{kl}\delta_{im}-\delta_{km}\delta_{il})A_lB_m (\stackrel{\rightarrow}{C} \textup{x} \stackrel{\rightarrow}{D})_k \\
&=&A_kB_i\epsilon_{kno}C_nD_0 - A_iB_k\epsilon_{kno}C_nD_0=\\
&=&B_i[\stackrel{\rightarrow}{A} , \stackrel{\rightarrow}{C} , \stackrel{\rightarrow}{D}]-A_i[\stackrel{\rightarrow}{B} , \stackrel{\rightarrow}{C} , \stackrel{\rightarrow}{D}]\\
&=&([\stackrel{\rightarrow}{A} , \stackrel{\rightarrow}{C} , \stackrel{\rightarrow}{D}] \stackrel{\rightarrow}{B} -
[\stackrel{\rightarrow}{B} , \stackrel{\rightarrow}{C} , \stackrel{\rightarrow}{D}] \stackrel{\rightarrow}{A})_i.
\end{eqnarray*}

\vspace{.1in}

{\bf \flushleft 4.} $(\stackrel{\rightarrow}{A} \textup{x} \stackrel{\rightarrow}{B})\cdot (\stackrel{\rightarrow}{B} \textup{x} \stackrel{\rightarrow}{C}) \textup{x} (\stackrel{\rightarrow}{C} \textup{x} \stackrel{\rightarrow}{A})= [\stackrel{\rightarrow}{A} , \stackrel{\rightarrow}{B} , \stackrel{\rightarrow}{C}] ^2$
{\flushleft \bf scalar=scalar}



\begin{eqnarray*}
(\stackrel{\rightarrow}{A} \textup{x} \stackrel{\rightarrow}{B})\cdot (\stackrel{\rightarrow}{B} \textup{x} \stackrel{\rightarrow}{C}) \textup{x} (\stackrel{\rightarrow}{C} \textup{x} \stackrel{\rightarrow}{A})&=&
\epsilon_{ijk}A_jB_k\epsilon_{ilm}(\stackrel{\rightarrow}{B} \textup{x} \stackrel{\rightarrow}{C})_l (\stackrel{\rightarrow}{C} \textup{x} \stackrel{\rightarrow}{A})_m\\
&=&
(\delta_{jl}\delta_{km}-\delta_{jm}\delta_{kl}) A_jB_k(\stackrel{\rightarrow}{B} \textup{x} \stackrel{\rightarrow}{C})_l (\stackrel{\rightarrow}{C} \textup{x} \stackrel{\rightarrow}{A})_m\\
&=&A_jB_k(\stackrel{\rightarrow}{B} \textup{x} \stackrel{\rightarrow}{C})_j (\stackrel{\rightarrow}{C} \textup{x} \stackrel{\rightarrow}{A})_k - A_jB_k(\stackrel{\rightarrow}{B} \textup{x} \stackrel{\rightarrow}{C})_k (\stackrel{\rightarrow}{C} \textup{x} \stackrel{\rightarrow}{A})_j \\
&=& \stackrel{\rightarrow}{A}\cdot(\stackrel{\rightarrow}{B} \textup{x} \stackrel{\rightarrow}{C})\stackrel{\rightarrow}{B}\cdot(\stackrel{\rightarrow}{C} \textup{x} \stackrel{\rightarrow}{A})-
\stackrel{\rightarrow}{A}\cdot(\stackrel{\rightarrow}{C} \textup{x} \stackrel{\rightarrow}{A})\stackrel{\rightarrow}{B}\cdot(\stackrel{\rightarrow}{B} \textup{x} \stackrel{\rightarrow}{C})\\
&=&[\stackrel{\rightarrow}{A} , \stackrel{\rightarrow}{B} , \stackrel{\rightarrow}{C}][\stackrel{\rightarrow}{B} , \stackrel{\rightarrow}{C} , \stackrel{\rightarrow}{A}]-0\\
&=&[\stackrel{\rightarrow}{A} , \stackrel{\rightarrow}{B} , \stackrel{\rightarrow}{C}]^2.
\end{eqnarray*}



\vspace{.1in}

{\bf \flushleft 5.}   $ \stackrel{\rightarrow}{A} \textup{x} (\stackrel{\rightarrow}{B}\textup{x} \stackrel{\rightarrow}{C}) +   \stackrel{\rightarrow}{B} \textup{x} (\stackrel{\rightarrow}{C}\textup{x} \stackrel{\rightarrow}{A}) +   \stackrel{\rightarrow}{C} \textup{x} (\stackrel{\rightarrow}{A}\textup{x} \stackrel{\rightarrow}{B})= \stackrel{\rightarrow}{0}$.
{\flushleft \bf vector=vector}
\begin{eqnarray*}
[\stackrel{\rightarrow}{A} \textup{x} (\stackrel{\rightarrow}{B}\textup{x} \stackrel{\rightarrow}{C}) +   \stackrel{\rightarrow}{B} \textup{x} (\stackrel{\rightarrow}{C}\textup{x} \stackrel{\rightarrow}{A}) +   \stackrel{\rightarrow}{C} \textup{x} (\stackrel{\rightarrow}{A}\textup{x} \stackrel{\rightarrow}{B})]_i & = &
\epsilon_{ijk} A_j (\stackrel{\rightarrow}{B}\textup{x} \stackrel{\rightarrow}{C})_k +
\epsilon_{ijk} B_j (\stackrel{\rightarrow}{C}\textup{x} \stackrel{\rightarrow}{A})_k +
\epsilon_{ijk} C_j (\stackrel{\rightarrow}{A}\textup{x} \stackrel{\rightarrow}{B})_k \\
&=&\epsilon_{ijk}\epsilon_{lmk}A_jB_lC_m + \epsilon_{ijk}\epsilon_{lmk}B_jC_lA_m + \epsilon_{ijk}\epsilon_{lmk}C_jA_lB_m\\
&=& (\delta_{il}\delta_{jm}-\delta_{im}\delta_{jl})[A_jB_lC_m+B_jC_lA_m+C_jA_lB_m]\\
&=&A_jB_iC_j - A_jB_jC_i+B_jC_iA_j-B_jC_jA_i+C_jA_iB_j-C_jA_jB_i\\
&=&[(\stackrel{\rightarrow}{A} \cdot \stackrel{\rightarrow}{C})\stackrel{\rightarrow}{B}-
(\stackrel{\rightarrow}{A} \cdot \stackrel{\rightarrow}{B})\stackrel{\rightarrow}{C}+
(\stackrel{\rightarrow}{A} \cdot \stackrel{\rightarrow}{B})\stackrel{\rightarrow}{C}-\\
&&
(\stackrel{\rightarrow}{B} \cdot \stackrel{\rightarrow}{C})\stackrel{\rightarrow}{A}+
(\stackrel{\rightarrow}{B} \cdot \stackrel{\rightarrow}{C})\stackrel{\rightarrow}{A}-
(\stackrel{\rightarrow}{C} \cdot \stackrel{\rightarrow}{A})\stackrel{\rightarrow}{B}]_i\\
&=&[\stackrel{\rightarrow}{0}]_i.
\end{eqnarray*}