% Chapter 1

\chapter{Tensor Notation and Vector Equations} % Main chapter title

\label{Chapter1} % For referencing the chapter elsewhere, use \ref{Chapter1} 

%----------------------------------------------------------------------------------------

% Define some commands to keep the formatting separated from the content 
\newcommand{\keyword}[1]{\textbf{#1}}
\newcommand{\tabhead}[1]{\textbf{#1}}
\newcommand{\code}[1]{\texttt{#1}}
\newcommand{\file}[1]{\texttt{\bfseries#1}}
\newcommand{\option}[1]{\texttt{\itshape#1}}

%----------------------------------------------------------------------------------------
\sectio{Tensor Notation for the Dot Product (Key formula:   $\stackrel{\rightarrow}{A} \cdot \stackrel{\rightarrow}{B} = A_iB_i $) }
\vspace{.2in}

Let $\stackrel{\rightarrow}{A}=A_1\stackrel{\rightarrow}{i }+A_2\stackrel{\rightarrow}{j }+A_3\stackrel{\rightarrow}{k }$ and
$\stackrel{\rightarrow}{B}=B_1\stackrel{\rightarrow}{i }+B_2\stackrel{\rightarrow}{j }+B_3\stackrel{\rightarrow}{k }$.

\begin{displaymath}
\stackrel{\rightarrow}{A} \cdot \stackrel{\rightarrow}{B} \stackrel{def}{=} \sum_{i=1}^3 \sum_{j=1}^3 \delta_{ij}A_iB_j =A_1B_1+A_2B_2+A_3B_3\hspace{.1in} \Rightarrow \hspace{.1in}  \delta_{ij} = \hspace{.1in}\rule{.25in}{.01in}\hspace{.1in} \textup{if}\hspace{.05in} i=j \hspace{.1in}\textup{and} \hspace{.2in} \delta_{ij}=\rule{.25in}{.01in} \hspace{.05in}\textup{if}\hspace{.05in} i\neq j.
\end{displaymath}

{\flushleft More} concisely, $\stackrel{\rightarrow}{A} \cdot \stackrel{\rightarrow}{B} = \sum_{i=1}^3 A_iB_i = A_iB_i$ where the last equality employs the following \emph{summation convention: If the same subscript appears in a term, that term must be summed over all values of the subscript.}

{\bf \flushleft Example:} Use tensor notation to show that the dot product is commutative.
{\flushleft Solution:}  $\stackrel{\rightarrow}{A} \cdot \stackrel{\rightarrow}{B} = A_iB_i = B_iA_i = \stackrel{\rightarrow}{B} \cdot \stackrel{\rightarrow}{A} $.


\section{ Tensor Notation for the Cross Product (Key formula: $[\stackrel{\rightarrow}{A} \textup{x} \stackrel{\rightarrow}{B}]_i = \epsilon_{ijk}A_jB_k $) }

\vspace{.1in}
 $[\stackrel{\rightarrow}{A} \textup{x} \stackrel{\rightarrow}{B}]_i \stackrel{def}{=} \sum_{j=1}^3\sum_{k=1}^3\epsilon_{ijk}A_jB_k \stackrel{summation convention}{=} \epsilon_{ijk}A_jB_k$

 {\flushleft Values of $\epsilon_{ijk}$}
  \begin{itemize}
 \item $\epsilon_{ijk}= \hspace{.1in}\rule{.25in}{.01in}$ if any of the subscripts are equal;
 \item $\epsilon_{ijk}= \epsilon_{jki}=\epsilon_{kij}$  (Subscripts may be permuted c\hspace{.1in}\rule{.5in}{.01in});
 \item  $\epsilon_{ijk}= -\epsilon_{jik}$ (Sign  c\hspace{.1in}\rule{.5in}{.01in} if two subscripts are interchanged);
 \end{itemize}
\vspace{.2in}

\section{Tensor Notation for the Scalar Triple Product (Key formula: $[\stackrel{\rightarrow}{A} , \stackrel{\rightarrow}{B} , \stackrel{\rightarrow}{C}]  =   \epsilon_{ijk}A_iB_jC_k$) }
\vspace{.1in}

$[\stackrel{\rightarrow}{A} , \stackrel{\rightarrow}{B} , \stackrel{\rightarrow}{C}]  \stackrel{def}{=}
\stackrel{\rightarrow}{A} \cdot (\stackrel{\rightarrow}{B} \textup{x} \stackrel{\rightarrow}{C})=
A_i (\stackrel{\rightarrow}{B} \textup{x} \stackrel{\rightarrow}{C})_i =
A_i \epsilon_{ijk}B_jC_k = \epsilon_{ijk}A_iB_jC_k$.

{\flushleft Note:} The absolute value of the scalar triple product (that is, $\mid  [\stackrel{\rightarrow}{A} , \stackrel{\rightarrow}{B} , \stackrel{\rightarrow}{C}]  \mid $) gives the volume of the parallelepiped determined by the vectors $\stackrel{\rightarrow}{A} , \stackrel{\rightarrow}{B}$ and  $\stackrel{\rightarrow}{C}$.


\section{Key Identity:  $\epsilon_{ikm}\epsilon_{psm} = \delta_{ip}\delta_{ks} -  \delta_{is}\delta_{kp}$.

\vspace{.2in}
{\flushleft 1.5 \bf Proving vector identities using tensor notation (Two Main Types!)}
\vspace{.1in}
{\flushleft \bf Type I: Scalar = Scalar}

{\bf \flushleft Example:} $ (\stackrel{\rightarrow}{A} \textup{x} \stackrel{\rightarrow}{B})\cdot \stackrel{\rightarrow}{C} = [\stackrel{\rightarrow}{A} , \stackrel{\rightarrow}{B} , \stackrel{\rightarrow}{C}] $

\vspace{.5in}

{\flushleft \bf Type II: Vector = Vector}

{\bf \flushleft Example:} $ \stackrel{\rightarrow}{A} \textup{x} (\stackrel{\rightarrow}{B}\textup{x} \stackrel{\rightarrow}{C})= ( \stackrel{\rightarrow}{A}\cdot \stackrel{\rightarrow}{C})\stackrel{\rightarrow}{B}  -   (\stackrel{\rightarrow}{A}\cdot \stackrel{\rightarrow}{B}) \stackrel{\rightarrow}{C}$


\section*{Homework 1}
{\flushleft Name:} \rule{1.5in}}\hspace{.02in}\rule{1.5in}{.01in}
\hspace{.02in}\rule{1.5in}{.01in}}

\vspace{.1in}

{\flushleft Use tensor notation to prove each identity. Begin by indicating whether the identity is of the form scalar=scalar or vector=vector.




{\bf \flushleft 1.}   $ \stackrel{\rightarrow}{A} \textup{x} \stackrel{\rightarrow}{B} = - (\stackrel{\rightarrow}{B} \textup{x} \stackrel{\rightarrow}{A})$.

\vspace{.5in}

{\bf \flushleft 2.} $(\stackrel{\rightarrow}{A} \textup{x} \stackrel{\rightarrow}{B})\cdot (\stackrel{\rightarrow}{C} \textup{x} \stackrel{\rightarrow}{D})=(\stackrel{\rightarrow}{A} \cdot \stackrel{\rightarrow}{C})(\stackrel{\rightarrow}{B} \cdot \stackrel{\rightarrow}{D} ) -
(\stackrel{\rightarrow}{A} \cdot \stackrel{\rightarrow}{D})(\stackrel{\rightarrow}{B} \cdot \stackrel{\rightarrow}{C} )$



\vspace{1.5in}
{\bf \flushleft 3.} $(\stackrel{\rightarrow}{A} \textup{x} \stackrel{\rightarrow}{B})\textup{x} (\stackrel{\rightarrow}{C} \textup{x} \stackrel{\rightarrow}{D})= [\stackrel{\rightarrow}{A} , \stackrel{\rightarrow}{C} , \stackrel{\rightarrow}{D}] \stackrel{\rightarrow}{B} -
[\stackrel{\rightarrow}{B} , \stackrel{\rightarrow}{C} , \stackrel{\rightarrow}{D}] \stackrel{\rightarrow}{A}$


\vspace{1.5in}

{\bf \flushleft 4.} $(\stackrel{\rightarrow}{A} \textup{x} \stackrel{\rightarrow}{B})\cdot (\stackrel{\rightarrow}{B} \textup{x} \stackrel{\rightarrow}{C}) \textup{x} (\stackrel{\rightarrow}{C} \textup{x} \stackrel{\rightarrow}{A})= [\stackrel{\rightarrow}{A} , \stackrel{\rightarrow}{B} , \stackrel{\rightarrow}{C}]^2$

\vspace{2in}

{\bf \flushleft 5.}   $ \stackrel{\rightarrow}{A} \textup{x} (\stackrel{\rightarrow}{B}\textup{x} \stackrel{\rightarrow}{C}) +   \stackrel{\rightarrow}{B} \textup{x} (\stackrel{\rightarrow}{C}\textup{x} \stackrel{\rightarrow}{A}) +   \stackrel{\rightarrow}{C} \textup{x} (\stackrel{\rightarrow}{A}\textup{x} \stackrel{\rightarrow}{B})= \stackrel{\rightarrow}{0}$.



\newpage

{\flushleft HW1}
{\bf \flushleft 1.}   $ \stackrel{\rightarrow}{A} \textup{x} \stackrel{\rightarrow}{B} = - (\stackrel{\rightarrow}{B} \textup{x} \stackrel{\rightarrow}{A})$.
{\flushleft \bf vector=vector}

 $[ \stackrel{\rightarrow}{A} \textup{x} \stackrel{\rightarrow}{B}]_i=
 \epsilon_{ijk}A_jB_k= - \epsilon_{ikj}B_kA_j = -[ \stackrel{\rightarrow}{B} \textup{x} \stackrel{\rightarrow}{A}]_i$
\vspace{.1in}

{\bf \flushleft 2.} $(\stackrel{\rightarrow}{A} \textup{x} \stackrel{\rightarrow}{B})\cdot (\stackrel{\rightarrow}{C} \textup{x} \stackrel{\rightarrow}{D})=(\stackrel{\rightarrow}{A} \cdot \stackrel{\rightarrow}{C})(\stackrel{\rightarrow}{B} \cdot \stackrel{\rightarrow}{D} ) -
(\stackrel{\rightarrow}{A} \cdot \stackrel{\rightarrow}{D})(\stackrel{\rightarrow}{B} \cdot \stackrel{\rightarrow}{C} )$
{\flushleft \bf scalar=scalar}
\begin{eqnarray*}
(\stackrel{\rightarrow}{A} \textup{x} \stackrel{\rightarrow}{B})
\cdot (\stackrel{\rightarrow}{C} \textup{x} \stackrel{\rightarrow}{D})&=&
\epsilon_{ijk}A_jB_k\epsilon_{ilm}C_lD_m\\
&=&\epsilon_{jki}\epsilon_{lmi}A_jB_kC_lD_m\\
&=&(\delta_{jl}\delta_{km}-\delta_{jm}\delta_{kl})A_jB_kC_lD_m\\
&=&A_jB_kC_jD_k-A_jB_kC_kD_j\\
&=&(\stackrel{\rightarrow}{A} \cdot \stackrel{\rightarrow}{C})(\stackrel{\rightarrow}{B} \cdot \stackrel{\rightarrow}{D} ) -
(\stackrel{\rightarrow}{A} \cdot \stackrel{\rightarrow}{D})(\stackrel{\rightarrow}{B} \cdot \stackrel{\rightarrow}{C} )
\end{eqnarray*}

\vspace{.1in}
{\bf \flushleft 3.} $(\stackrel{\rightarrow}{A} \textup{x} \stackrel{\rightarrow}{B})\textup{x} (\stackrel{\rightarrow}{C} \textup{x} \stackrel{\rightarrow}{D})= [\stackrel{\rightarrow}{A} , \stackrel{\rightarrow}{C} , \stackrel{\rightarrow}{D}] \stackrel{\rightarrow}{B} -
[\stackrel{\rightarrow}{B} , \stackrel{\rightarrow}{C} , \stackrel{\rightarrow}{D}] \stackrel{\rightarrow}{A}$
{\flushleft \bf vector=vector}
\begin{eqnarray*}
[(\stackrel{\rightarrow}{A} \textup{x} \stackrel{\rightarrow}{B})\textup{x} (\stackrel{\rightarrow}{C} \textup{x} \stackrel{\rightarrow}{D})]_i&=&
\epsilon_{ijk}(\stackrel{\rightarrow}{A} \textup{x} \stackrel{\rightarrow}{B})_j (\stackrel{\rightarrow}{C} \textup{x} \stackrel{\rightarrow}{D})_k\\
&=&\epsilon_{ijk}\epsilon_{jlm}A_lB_m (\stackrel{\rightarrow}{C} \textup{x} \stackrel{\rightarrow}{D})_k\\
&=&\epsilon_{kij}\epsilon_{lmj}A_lB_m (\stackrel{\rightarrow}{C} \textup{x} \stackrel{\rightarrow}{D})_k\\
&=&(\delta_{kl}\delta_{im}-\delta_{km}\delta_{il})A_lB_m (\stackrel{\rightarrow}{C} \textup{x} \stackrel{\rightarrow}{D})_k \\
&=&A_kB_i\epsilon_{kno}C_nD_0 - A_iB_k\epsilon_{kno}C_nD_0=\\
&=&B_i[\stackrel{\rightarrow}{A} , \stackrel{\rightarrow}{C} , \stackrel{\rightarrow}{D}]-A_i[\stackrel{\rightarrow}{B} , \stackrel{\rightarrow}{C} , \stackrel{\rightarrow}{D}]\\
&=&([\stackrel{\rightarrow}{A} , \stackrel{\rightarrow}{C} , \stackrel{\rightarrow}{D}] \stackrel{\rightarrow}{B} -
[\stackrel{\rightarrow}{B} , \stackrel{\rightarrow}{C} , \stackrel{\rightarrow}{D}] \stackrel{\rightarrow}{A})_i.
\end{eqnarray*}

\vspace{.1in}

{\bf \flushleft 4.} $(\stackrel{\rightarrow}{A} \textup{x} \stackrel{\rightarrow}{B})\cdot (\stackrel{\rightarrow}{B} \textup{x} \stackrel{\rightarrow}{C}) \textup{x} (\stackrel{\rightarrow}{C} \textup{x} \stackrel{\rightarrow}{A})= [\stackrel{\rightarrow}{A} , \stackrel{\rightarrow}{B} , \stackrel{\rightarrow}{C}] ^2$
{\flushleft \bf scalar=scalar}



\begin{eqnarray*}
(\stackrel{\rightarrow}{A} \textup{x} \stackrel{\rightarrow}{B})\cdot (\stackrel{\rightarrow}{B} \textup{x} \stackrel{\rightarrow}{C}) \textup{x} (\stackrel{\rightarrow}{C} \textup{x} \stackrel{\rightarrow}{A})&=&
\epsilon_{ijk}A_jB_k\epsilon_{ilm}(\stackrel{\rightarrow}{B} \textup{x} \stackrel{\rightarrow}{C})_l (\stackrel{\rightarrow}{C} \textup{x} \stackrel{\rightarrow}{A})_m\\
&=&
(\delta_{jl}\delta_{km}-\delta_{jm}\delta_{kl}) A_jB_k(\stackrel{\rightarrow}{B} \textup{x} \stackrel{\rightarrow}{C})_l (\stackrel{\rightarrow}{C} \textup{x} \stackrel{\rightarrow}{A})_m\\
&=&A_jB_k(\stackrel{\rightarrow}{B} \textup{x} \stackrel{\rightarrow}{C})_j (\stackrel{\rightarrow}{C} \textup{x} \stackrel{\rightarrow}{A})_k - A_jB_k(\stackrel{\rightarrow}{B} \textup{x} \stackrel{\rightarrow}{C})_k (\stackrel{\rightarrow}{C} \textup{x} \stackrel{\rightarrow}{A})_j \\
&=& \stackrel{\rightarrow}{A}\cdot(\stackrel{\rightarrow}{B} \textup{x} \stackrel{\rightarrow}{C})\stackrel{\rightarrow}{B}\cdot(\stackrel{\rightarrow}{C} \textup{x} \stackrel{\rightarrow}{A})-
\stackrel{\rightarrow}{A}\cdot(\stackrel{\rightarrow}{C} \textup{x} \stackrel{\rightarrow}{A})\stackrel{\rightarrow}{B}\cdot(\stackrel{\rightarrow}{B} \textup{x} \stackrel{\rightarrow}{C})\\
&=&[\stackrel{\rightarrow}{A} , \stackrel{\rightarrow}{B} , \stackrel{\rightarrow}{C}][\stackrel{\rightarrow}{B} , \stackrel{\rightarrow}{C} , \stackrel{\rightarrow}{A}]-0\\
&=&[\stackrel{\rightarrow}{A} , \stackrel{\rightarrow}{B} , \stackrel{\rightarrow}{C}]^2.
\end{eqnarray*}



\vspace{.1in}

{\bf \flushleft 5.}   $ \stackrel{\rightarrow}{A} \textup{x} (\stackrel{\rightarrow}{B}\textup{x} \stackrel{\rightarrow}{C}) +   \stackrel{\rightarrow}{B} \textup{x} (\stackrel{\rightarrow}{C}\textup{x} \stackrel{\rightarrow}{A}) +   \stackrel{\rightarrow}{C} \textup{x} (\stackrel{\rightarrow}{A}\textup{x} \stackrel{\rightarrow}{B})= \stackrel{\rightarrow}{0}$.
{\flushleft \bf vector=vector}
\begin{eqnarray*}
[\stackrel{\rightarrow}{A} \textup{x} (\stackrel{\rightarrow}{B}\textup{x} \stackrel{\rightarrow}{C}) +   \stackrel{\rightarrow}{B} \textup{x} (\stackrel{\rightarrow}{C}\textup{x} \stackrel{\rightarrow}{A}) +   \stackrel{\rightarrow}{C} \textup{x} (\stackrel{\rightarrow}{A}\textup{x} \stackrel{\rightarrow}{B})]_i & = &
\epsilon_{ijk} A_j (\stackrel{\rightarrow}{B}\textup{x} \stackrel{\rightarrow}{C})_k +
\epsilon_{ijk} B_j (\stackrel{\rightarrow}{C}\textup{x} \stackrel{\rightarrow}{A})_k +
\epsilon_{ijk} C_j (\stackrel{\rightarrow}{A}\textup{x} \stackrel{\rightarrow}{B})_k \\
&=&\epsilon_{ijk}\epsilon_{lmk}A_jB_lC_m + \epsilon_{ijk}\epsilon_{lmk}B_jC_lA_m + \epsilon_{ijk}\epsilon_{lmk}C_jA_lB_m\\
&=& (\delta_{il}\delta_{jm}-\delta_{im}\delta_{jl})[A_jB_lC_m+B_jC_lA_m+C_jA_lB_m]\\
&=&A_jB_iC_j - A_jB_jC_i+B_jC_iA_j-B_jC_jA_i+C_jA_iB_j-C_jA_jB_i\\
&=&[(\stackrel{\rightarrow}{A} \cdot \stackrel{\rightarrow}{C})\stackrel{\rightarrow}{B}-
(\stackrel{\rightarrow}{A} \cdot \stackrel{\rightarrow}{B})\stackrel{\rightarrow}{C}+
(\stackrel{\rightarrow}{A} \cdot \stackrel{\rightarrow}{B})\stackrel{\rightarrow}{C}-\\
&&
(\stackrel{\rightarrow}{B} \cdot \stackrel{\rightarrow}{C})\stackrel{\rightarrow}{A}+
(\stackrel{\rightarrow}{B} \cdot \stackrel{\rightarrow}{C})\stackrel{\rightarrow}{A}-
(\stackrel{\rightarrow}{C} \cdot \stackrel{\rightarrow}{A})\stackrel{\rightarrow}{B}]_i\\
&=&[\stackrel{\rightarrow}{0}]_i.
\end{eqnarray*}